% !TEX root = ../../MakeBeamer.tex
\title[Correlations]{Linear Regression: Correlations}
\date{}


\def\askone{Show that the regression $R^2$ in the regression of $Y$ on $X$ is the squared value of the sample correlation between $X$ and $Y$. That is, show that $R^2=r^2_{XY}$.}

\begin{document}


\inputfile{../Section-Cover-Problems}


%%%%%%%%%%%%%%%%%%%%%%%%%%%%%%%%%%%%%%%%%%%%%%%%%%%%%%%%%
\begin{frame}[fragile]
\frametitle{Correlations}
\exercise{Stock \& Watson, Introduction (4th), Chapter~4, Exercise~12.}

\begin{enumerate}\setcounter{enumi}{0}

\item \askone

\begin{answer}
Pearson's sample correlation coefficient $r_{XY}$ (population is denoted $\rho_{XY}$) is
\begin{align*}
r_{XY} 
    = \frac{s_{XY}}{s_{X}s_{Y}}
\end{align*}

The OLS estimator may be written:
\begin{align*}
\hat{\beta}_{1} 
    = \frac{\sum_{i=1}^{n}(X_{i}-\mean{X})(Y_{i}-\mean{Y})}{\sum_{i=1}^{n}(X_{i}-\mean{X})^{2}}
    = \frac{s_{XY}}{s_{X}^2}
\end{align*}
where $s_{XY}$ denotes the sample covariance and $s_{X}^2$ denotes the variance, $s_{XY}=s_{X}^2$. The proof of this is standard and follows from minimizing the sum of squared residuals of the regression of $Y$ on $X$. 
\begin{comment}
If you were expected to show it, I think the question would be more explicit.
It follows that
\begin{align*}
r_{XY} 
    = \frac{s_{X,Y}}{s_{X}s_{Y}}
    = \frac{s_{X,Y}}{s_{X}s_{Y}}\frac{s_{X}}{s_{X}}
    = \frac{s_{X,Y}}{s_{X}^2}\frac{s_{X}}{s_{Y}}
    = \hat{\beta}_{1} \frac{s_{X}}{s_{Y}}
\end{align*}
\end{comment}

The coefficient of determination of the regression of $Y$ on $X$ is
\begin{align*}
R^{2}
  = 1 - \frac{\sum_{i=1}^{n}\hat{u}_{i}^2}{\sum_{i=1}^{n}(Y_{i}-\mean{Y})^2}
  = 1 - \frac{\sum_{i=1}^{n}(Y_{i}-\hat{\beta}_{0}-\hat{\beta}_{1}X_{i})^2}{s_{YY}}
\end{align*}
\end{answer}

\end{enumerate}
\end{frame}
%%%%%%%%%%%%%%%%%%%%%%%%%%%%%%%%%%%%%%%%%%%%%%%%%%%%%%%%%


%%%%%%%%%%%%%%%%%%%%%%%%%%%%%%%%%%%%%%%%%%%%%%%%%%%%%%%%%
\begin{frame}
\frametitle{Correlations}

\begin{enumerate}\setcounter{enumi}{0}

\item \askone

\begin{answer}
\begin{align*}
\hat{\beta}_{0}
     = \mean{Y} - \hat{\beta}_{1} \mean{X}
\implies
& \sum_{i=1}^{n}(Y_{i}-\hat{\beta}_{0}-\hat{\beta}_{1}X_{i})^2
     = \sum_{i=1}^{n}[(Y_{i}-\mean{Y})-\hat{\beta}_{1}(X_{i}-\mean{X})])^2\\
    & = \sum_{i=1}^{n}(Y_{i}-\mean{Y})^2
       -2\hat{\beta}_{1}\sum_{i=1}^{n}(X_{i}-\mean{X})(Y_{i}-\mean{Y})
       + \hat{\beta}_{1}^2\sum_{i=1}^{n}(X_{i}-\mean{X})^2\\
    & = s_{YY} -2\hat{\beta}_{1} s_{XY} + \hat{\beta}_{1}^2 s_{XX}
\end{align*}
Plugging the above into the coefficient of determination:
\begin{align*}
R^{2} 
    &  = 1 - \frac{s_{YY} -2\hat{\beta}_{1} s_{XY} + \hat{\beta}_{1}^2 s_{XX}}{s_{YY}} 
      = 2\hat{\beta}_{1} \frac{s_{XY}}{s_{YY}} - \hat{\beta}_{1}^2 \frac{s_{XX}}{s_{YY}}\\
    & = 2 \frac{s_{XY}}{s_{X}^2}\frac{s_{XY}}{s_{YY}} 
         - \left(\frac{s_{XY}}{s_{X}^2}\right)^2 \frac{s_{XX}}{s_{YY}}
      = \frac{s_{XY}^2}{s_{X}^2\,s_{Y}^2} 
      = r_{XY}^2
\end{align*}
\end{answer}

\end{enumerate}
\end{frame}
%%%%%%%%%%%%%%%%%%%%%%%%%%%%%%%%%%%%%%%%%%%%%%%%%%%%%%%%%


%%%%%%%%%%%%%%%%%%%%%%%%%%%%%%%%%%%%%%%%%%%%%%%%%%%%%%%%%
\begin{frame}
\frametitle{Correlations}

\begin{enumerate}\setcounter{enumi}{1}

\item Show that the $R^2$ from the regression of $Y$ on $X$ is the same as the $R^2$ from the regression of $X$ on $Y$.

\begin{answer}
Since we have shown that $R^2=r^2_{XY}$, it follows from $s_{XY}=s_{YX}$:
\begin{align*}
R^{2} ~\text{of $Y$ on $X$}
  = r_{XY}^2
  = \frac{s_{XY}}{s_{X}s_{Y}}
  = \frac{s_{YX}}{s_{Y}s_{X}}
  = r_{YX}^2
  = R^{2} ~\text{of $X$ on $Y$}
\end{align*}
\end{answer}


\end{enumerate}
\end{frame}
%%%%%%%%%%%%%%%%%%%%%%%%%%%%%%%%%%%%%%%%%%%%%%%%%%%%%%%%%


%%%%%%%%%%%%%%%%%%%%%%%%%%%%%%%%%%%%%%%%%%%%%%%%%%%%%%%%%
\begin{frame}
\frametitle{Correlations}

\begin{enumerate}\setcounter{enumi}{2}

\item Show that $\hat{\beta}_1=r_{XY}(s_{Y}/s_{X})$, where $r_{XY}$ is the sample correlation between $X$ and $Y$, and $s_X$ and $s_Y$ are the sample standard deviations of $X$ and $Y$.

\begin{answer}
We've done most of the work already:
\begin{align*}
\hat{\beta}_{1}
    = \frac{s_{XY}}{s_{X}^2}
    = \frac{r_{XY} s_{X} s_{Y}}{s_{X}^2}
    = \frac{r_{XY} s_{Y}}{s_{X}}
\end{align*}
\end{answer}

\end{enumerate}
\end{frame}
%%%%%%%%%%%%%%%%%%%%%%%%%%%%%%%%%%%%%%%%%%%%%%%%%%%%%%%%%


\end{document}